encode.v
@@ -6,26 +6,95 @@ Import ListNotations.
 Check (1,2).
 Check pair nat nat.
 Definition tag_opcode_assoc :=
-  list (tag * (list bool)).
+  list (tag * nat).
 
 Scheme Equality for list.
 Check list_beq.
 
-Fixpoint get_opcode (t : tag) (l : tag_opcode_assoc) : option (list bool) :=
+
+
+
+
+
+(* actually this is a good name for this function :p *)
+Fixpoint lookup (t : tag) (l : tag_opcode_assoc) : option nat :=
   match l with
     | [] => None
-    | (t',r) :: tl => if tag_beq t t'
-                      then Some r
-                      else get_opcode t tl
+    | (t',n) :: tl => if tag_beq t t'
+                      then Some n
+                      else lookup t tl
+  end.
+(* actually this is a good name for this function :p *)
+Fixpoint lookdown (n : nat) (l : tag_opcode_assoc) : option tag :=
+  match l with
+    | [] => None
+    | (t,n') :: tl => if  eqb n n'
+                      then Some t
+                      else lookdown n tl
   end.
 
-Fixpoint get_tag (o : list bool) (l : tag_opcode_assoc) : option tag :=
-  match l with
-    | [] => None
-    | (t,o') :: tl => if list_beq bool Bool.eqb o o'
-                      then Some t
-                      else get_tag o tl
-  end.
+(* this table is an association list of type tag_opcode_assoc with every associations that can be made in our langage *)
+Definition encdec : tag_opcode_assoc := [(tag_n(ADD),1);(tag_n(AND),2);(tag_i(ADD_I),3);(tag_i(AND_I),4)].
+
+Theorem lookup_encdec : forall (t : tag), exists n,
+                          lookup t encdec = Some n.
+Proof.
+  destruct t.
+  -destruct t.
+   +simpl. exists 1. reflexivity.
+   +simpl. exists 2. reflexivity.
+  -destruct t.
+   +simpl. exists 3. reflexivity.
+   +simpl. exists 4. reflexivity.
+Qed.
+
+
+(* TODO : i know that i can refoctor this proof but at the first try i didn't succeed so will try later *)
+Theorem look_up_down_encdec : forall (n : nat) (t : tag),
+                                lookup t encdec = Some n -> lookdown n encdec = Some t.
+Proof.
+  assert (I : forall (n : nat) (t : tag), lookup t encdec = Some n -> lookdown n encdec = Some t).
+  {
+    destruct t.
+    -destruct t.
+     +intros H.
+      simpl in H.
+      inversion H.
+      reflexivity.
+     +intros H.
+      simpl in H.
+      inversion H.
+      reflexivity.
+    -destruct t.
+     +intros H.
+      simpl in H.
+      inversion H.
+      reflexivity.
+     +intros H.
+      simpl in H.
+      inversion H.
+      reflexivity.
+  }
+  exact I.
+Qed.
+
+(* if i wan't it's very easy to proof with forall t exists n but this theorem is better and actually it's true *)
+Theorem look_down_up_encdec : forall (n : nat) (t : tag),
+                                lookdown n encdec = Some t -> lookup t encdec = Some n.
+Proof.
+  assert (I : forall (n : nat) (t : tag), lookdown n encdec = Some t -> lookup t encdec = Some n).
+  {
+    intros n t.
+    destruct (lookdown n encdec).
+    {destruct t0.
+     -destruct t0.
+      +intros H.
+       simpl in H.
+       inversion H.
+       
+    } 
+  }
+
 
 
 
